steel/Zeta.Steel.AggregateEpochHashes.fsti
@@ -12,48 +12,29 @@ module U16 = FStar.UInt16
 module U32 = FStar.UInt32
 module U64 = FStar.UInt64
 open Zeta.Steel.FormatsManual
-module IArray = Zeta.Steel.IArray
+module EpochMap = Zeta.Steel.EpochMap
 module T = Zeta.Steel.FormatsManual
 module M = Zeta.Steel.ThreadStateModel
 module HA = Zeta.Steel.HashAccumulator
 open Zeta.Steel.Util
 module MR = Steel.ST.MonotonicReference
 module TLM = Zeta.Steel.ThreadLogMap
+open Zeta.Steel.EpochHashes
 #push-options "--ide_id_info_off"
 
 /// Initializer for an IArray
 val epoch_hash_size : U32.t
 
-noeq
-type epoch_hashes_t = {
-  hadd: HA.ha;
-  hevict: HA.ha;
-}
-
-let epoch_hashes_repr = IArray.repr M.epoch_id M.epoch_hash
-let epoch_id_hash (x:M.epoch_id) : U32.t = x
-let epoch_hash_perm (k:M.epoch_id)
-                    (v:epoch_hashes_t)
-                    (c:M.epoch_hash) =
-    HA.ha_val v.hadd c.hadd `star`
-    HA.ha_val v.hevict c.hevict
-
-let all_epoch_hashes =
-  IArray.tbl
-    #M.epoch_id
-    #epoch_hashes_t
-    #M.epoch_hash
-    epoch_id_hash
-    epoch_hash_perm
-
 let tid_bitmap = Seq.lseq bool (U32.v n_threads)
+let epoch_hashes_repr = EpochMap.repr M.epoch_hash
+let epoch_bitmaps_repr = EpochMap.repr tid_bitmap
+
+let all_epoch_hashes = EpochMap.tbl epoch_hash_perm
+
 let epoch_tid_bitmaps =
-  IArray.tbl
-    #M.epoch_id
-    #(larray bool n_threads)
-    #tid_bitmap
-    epoch_id_hash
-    (fun i -> array_pts_to)
+  EpochMap.tbl #(larray bool n_threads)
+               #tid_bitmap
+               (fun i -> array_pts_to)
 
 let is_epoch_verified (tsm:M.thread_state_model) (eid:M.epoch_id) =
   U32.v tsm.M.last_verified_epoch >= U32.v eid
@@ -113,9 +94,10 @@ let all_contributions_are_accurate (global:epoch_hashes_repr)
   = forall (e:M.epoch_id). Map.sel global e == aggregate_all_threads_epoch_hashes e mlogs_v
 
 let all_ones = Seq.create (U32.v n_threads) true
+let all_zeroes = Seq.create (U32.v n_threads) false
 
 let max_certified_epoch_is (global:epoch_hashes_repr)
-                           (bitmaps: IArray.repr M.epoch_id tid_bitmap)
+                           (bitmaps:epoch_bitmaps_repr)
                            (max:M.epoch_id)
   : prop
   = forall (e:M.epoch_id).
@@ -127,7 +109,7 @@ let max_certified_epoch_is (global:epoch_hashes_repr)
 let epoch_is_complete (mlogs_v:all_processed_entries) (e:M.epoch_id)
   = forall tid. is_epoch_verified (tsm_of_log mlogs_v tid) e
 
-let per_thread_bitmap_and_max (bitmaps: IArray.repr M.epoch_id tid_bitmap)
+let per_thread_bitmap_and_max (bitmaps:epoch_bitmaps_repr)
                               (max:M.epoch_id)
                               (all_logs:all_processed_entries)
                               (tid:tid)
@@ -138,14 +120,13 @@ let per_thread_bitmap_and_max (bitmaps: IArray.repr M.epoch_id tid_bitmap)
       Seq.index (Map.sel bitmaps eid) (U16.v tid) == is_epoch_verified tsm eid)
 
 let hashes_bitmaps_max_ok (hashes:epoch_hashes_repr)
-                          (bitmaps: IArray.repr M.epoch_id tid_bitmap)
+                          (bitmaps:epoch_bitmaps_repr)
                           (max:M.epoch_id)
                           (mlogs_v:all_processed_entries)
  : prop
  = all_contributions_are_accurate hashes mlogs_v /\
    max_certified_epoch_is hashes bitmaps max /\
    (forall tid. per_thread_bitmap_and_max bitmaps max mlogs_v tid)
-
 
 
 [@@__reduce__]
@@ -157,8 +138,8 @@ let lock_inv_body (hashes : all_epoch_hashes)
                   (bitmaps:_)
                   (max:_)
                   (mlogs_v:all_processed_entries)
-  = IArray.full_perm hashes hashes_v `star`
-    IArray.full_perm tid_bitmaps bitmaps `star`
+  = EpochMap.full_perm hashes M.init_epoch_hash hashes_v `star`
+    EpochMap.full_perm tid_bitmaps all_zeroes bitmaps `star`
     R.pts_to max_certified_epoch full max `star`
     TLM.global_anchor mlogs (map_of_seq mlogs_v) `star`
     pure (hashes_bitmaps_max_ok hashes_v bitmaps max mlogs_v)
@@ -184,7 +165,6 @@ type aggregate_epoch_hashes = {
      lock: cancellable_lock (lock_inv hashes tid_bitmaps max_certified_epoch mlogs)
 }
 #push-options "--print_effect_args"
-module EHT = Steel.ST.EphemeralHashtbl
 
 let check_all_ones (#e:Ghost.erased _)
                    (a:larray bool n_threads)
@@ -195,13 +175,13 @@ let check_all_ones (#e:Ghost.erased _)
     (ensures fun b -> b <==> (reveal e == all_ones))
   = admit__()
 
-let return_borrows (#k:eqtype) (#v:Type0) (b:IArray.borrows k v) (i:k) (x:v)
+let return_borrows (#v:Type0) (b:EpochMap.borrows v) (i:M.epoch_id) (x:v)
   : Lemma (requires ~(PartialMap.contains i b))
           (ensures (PartialMap.remove i (PartialMap.upd i x b) `PartialMap.equal` b))
           [SMTPat (PartialMap.remove i (PartialMap.upd i x b))]
   = ()
 
-let return_map (#k:eqtype) (#v:Type0) (m:IArray.repr k v) (i:k)
+let return_map (#v:Type0) (m:EpochMap.repr v) (i:M.epoch_id)
   : Lemma (ensures (Map.upd m i (Map.sel m i) `Map.equal` m))
           [SMTPat (Map.upd m i (Map.sel m i))]
   = ()
@@ -210,41 +190,41 @@ let check_bitmap_for_epoch (#bm:erased _)
                            (tid_bitmaps: epoch_tid_bitmaps)
                            (e:M.epoch_id)
   : ST bool
-    (IArray.full_perm tid_bitmaps bm)
-    (fun b -> IArray.full_perm tid_bitmaps bm)
+    (EpochMap.full_perm tid_bitmaps all_zeroes bm)
+    (fun b -> EpochMap.full_perm tid_bitmaps all_zeroes bm)
     (requires True)
     (ensures fun b -> b ==> Map.sel bm e == all_ones)
-  = let res = IArray.get tid_bitmaps e in
+  = let res = EpochMap.get tid_bitmaps e in
     match res with
-    | EHT.Present a ->
-      rewrite (IArray.get_post bm IArray.empty_borrows tid_bitmaps e res)
-              (IArray.perm tid_bitmaps bm (PartialMap.upd e a IArray.empty_borrows) `star`
+    | EpochMap.Found a ->
+      rewrite (EpochMap.get_post all_zeroes bm EpochMap.empty_borrows tid_bitmaps e res)
+              (EpochMap.perm tid_bitmaps all_zeroes bm (PartialMap.upd e a EpochMap.empty_borrows) `star`
                array_pts_to a (Map.sel bm e));
       let b = check_all_ones a in
-      IArray.ghost_put tid_bitmaps e a _;
+      EpochMap.ghost_put tid_bitmaps e a _;
       return b
 
     | _ ->
-      rewrite (IArray.get_post bm IArray.empty_borrows tid_bitmaps e res)
-              (IArray.full_perm tid_bitmaps bm);
+      rewrite (EpochMap.get_post all_zeroes bm EpochMap.empty_borrows tid_bitmaps e res)
+              (EpochMap.full_perm tid_bitmaps all_zeroes bm);
       return false
 
 
-let check_hash_equality_for_epoch (#hashes_v:erased (IArray.repr M.epoch_id M.epoch_hash))
+let check_hash_equality_for_epoch (#hashes_v:erased epoch_hashes_repr)
                                   (hashes:all_epoch_hashes)
                                   (e:M.epoch_id)
   : ST bool
-    (IArray.full_perm hashes hashes_v)
-    (fun _ -> IArray.full_perm hashes hashes_v)
+    (EpochMap.full_perm hashes M.init_epoch_hash hashes_v)
+    (fun _ -> EpochMap.full_perm hashes M.init_epoch_hash hashes_v)
     (requires True)
     (ensures fun b ->
       let ha = Map.sel hashes_v e in
       b ==> ha.hadd == ha.hevict)
-  = let res = IArray.get hashes e in
+  = let res = EpochMap.get hashes e in
     match res with
-    | EHT.Present ehs ->
-      rewrite (IArray.get_post hashes_v IArray.empty_borrows hashes e res)
-              (IArray.perm hashes hashes_v (PartialMap.upd e ehs IArray.empty_borrows) `star`
+    | EpochMap.Found ehs ->
+      rewrite (EpochMap.get_post M.init_epoch_hash hashes_v EpochMap.empty_borrows hashes e res)
+              (EpochMap.perm hashes M.init_epoch_hash hashes_v (PartialMap.upd e ehs EpochMap.empty_borrows) `star`
                epoch_hash_perm e ehs (Map.sel hashes_v e));
       rewrite (epoch_hash_perm e ehs (Map.sel hashes_v e)) //TODO: mark epoch_hash_perm reduce
               (HA.ha_val ehs.hadd (Map.sel hashes_v e).hadd `star`
@@ -253,16 +233,16 @@ let check_hash_equality_for_epoch (#hashes_v:erased (IArray.repr M.epoch_id M.ep
       rewrite (HA.ha_val ehs.hadd (Map.sel hashes_v e).hadd `star`
                HA.ha_val ehs.hevict (Map.sel hashes_v e).hevict)
               (epoch_hash_perm e ehs (Map.sel hashes_v e));
-      IArray.ghost_put hashes e ehs _;
+      EpochMap.ghost_put hashes e ehs _;
       return  b
 
     | _ ->
-      rewrite (IArray.get_post hashes_v IArray.empty_borrows hashes e res)
-              (IArray.full_perm hashes hashes_v);
+      rewrite (EpochMap.get_post M.init_epoch_hash hashes_v EpochMap.empty_borrows hashes e res)
+              (EpochMap.full_perm hashes M.init_epoch_hash hashes_v);
       return false
 
-let epoch_ready_if_bitmap_set (hashes:IArray.repr _ _)
-                              (bitmaps:_)
+let epoch_ready_if_bitmap_set (hashes:epoch_hashes_repr)
+                              (bitmaps:epoch_bitmaps_repr)
                               (max:_)
                               (mlogs_v:_)
                               (e:M.epoch_id)
@@ -304,14 +284,14 @@ let try_increment_max (#hashes_v:erased _)
                       (bitmaps: epoch_tid_bitmaps)
                       (max:R.ref M.epoch_id)
   : STT bool
-    (IArray.full_perm hashes hashes_v `star`
-     IArray.full_perm bitmaps bitmaps_v `star`
+    (EpochMap.full_perm hashes M.init_epoch_hash hashes_v `star`
+     EpochMap.full_perm bitmaps all_zeroes bitmaps_v `star`
      exists_ (fun max_v ->
        R.pts_to max full max_v `star`
        pure (hashes_bitmaps_max_ok hashes_v bitmaps_v max_v mlogs_v)))
     (fun b ->
-      IArray.full_perm hashes hashes_v `star`
-      IArray.full_perm bitmaps bitmaps_v `star`
+      EpochMap.full_perm hashes M.init_epoch_hash hashes_v `star`
+      EpochMap.full_perm bitmaps all_zeroes bitmaps_v `star`
       exists_ (fun (max_v':M.epoch_id) ->
         R.pts_to max full max_v' `star`
         pure (hashes_bitmaps_max_ok hashes_v bitmaps_v max_v' mlogs_v)))
@@ -350,25 +330,25 @@ let try_increment_max (#hashes_v:erased _)
           intro_exists e' (fun max_v' ->
             R.pts_to max full max_v' `star`
             pure (hashes_bitmaps_max_ok hashes_v bitmaps_v max_v' mlogs_v));
-          return true
+           return true
         )
       )
 
-let try_advance_max (#hashes_v:erased _)
-                    (#bitmaps_v:erased _)
+let try_advance_max (#hashes_v:erased epoch_hashes_repr)
+                    (#bitmaps_v:erased epoch_bitmaps_repr)
                     (#max_v:erased _)
                     (#mlogs_v:erased _)
                     (hashes: all_epoch_hashes)
                     (bitmaps: epoch_tid_bitmaps)
                     (max:R.ref M.epoch_id)
   : STT M.epoch_id
-    (IArray.full_perm hashes hashes_v `star`
-     IArray.full_perm bitmaps bitmaps_v `star`
+    (EpochMap.full_perm hashes M.init_epoch_hash hashes_v `star`
+     EpochMap.full_perm bitmaps all_zeroes bitmaps_v `star`
      R.pts_to max full max_v `star`
      pure (hashes_bitmaps_max_ok hashes_v bitmaps_v max_v mlogs_v))
     (fun max_v' ->
-      IArray.full_perm hashes hashes_v `star`
-      IArray.full_perm bitmaps bitmaps_v `star`
+      EpochMap.full_perm hashes M.init_epoch_hash hashes_v `star`
+      EpochMap.full_perm bitmaps all_zeroes bitmaps_v `star`
       R.pts_to max full max_v' `star`
       pure (hashes_bitmaps_max_ok hashes_v bitmaps_v max_v' mlogs_v))
   = intro_exists_erased max_v (fun max_v ->
@@ -381,8 +361,8 @@ let try_advance_max (#hashes_v:erased _)
     intro_pure _;
     return max
 
-let release_lock (#hv:erased _)
-                 (#bitmaps:erased _)
+let release_lock (#hv:erased epoch_hashes_repr)
+                 (#bitmaps:erased epoch_bitmaps_repr)
                  (#max:erased _)
                  (#mlogs_v:erased _)
                  (#hashes : all_epoch_hashes)
