steel/Zeta.Steel.EpochHashes.fsti
@@ -1,0 +1,18 @@
+module Zeta.Steel.EpochHashes
+open Steel.ST.Util
+open Zeta.Steel.Util
+module M = Zeta.Steel.ThreadStateModel
+module HA = Zeta.Steel.HashAccumulator
+
+
+noeq
+type epoch_hashes_t = {
+  hadd: HA.ha;
+  hevict: HA.ha;
+}
+
+let epoch_hash_perm (k:M.epoch_id)
+                    (v:epoch_hashes_t)
+                    (c:M.epoch_hash) =
+    HA.ha_val v.hadd c.hadd `star`
+    HA.ha_val v.hevict c.hevict
