steel/Zeta.Steel.EpochMap.fsti
@@ -1,0 +1,178 @@
+module Zeta.Steel.EpochMap
+open Steel.ST.Util
+open Zeta.Steel.Util
+module M = Zeta.Steel.ThreadStateModel
+module G = FStar.Ghost
+module Set = FStar.Set
+module Map = FStar.Map
+module U32 = FStar.UInt32
+
+val tbl (#v:Type)
+        (#c:Type) 
+        (vp:M.epoch_id -> v -> c -> vprop)
+    : Type0
+
+let repr (a:Type)
+  : Type0
+  = m:Map.t M.epoch_id a {
+      Map.domain m `Set.equal` Set.complement Set.empty
+    }
+
+let borrows (a:Type)
+  : Type0
+  = FStar.PartialMap.t M.epoch_id a
+
+let empty_borrows #a
+  : borrows a
+  = PartialMap.empty M.epoch_id a
+
+(*
+  One representation for this is a pair containing an
+    1. an EHT
+    2. a high-water-mark, a concrete epoch_id ref
+
+  with an invariant stating that for all 
+  
+    epoch_id greater than the high-water-mark
+    the value of the map associated with that epoch id
+    is the default_value
+
+  Additionally, if an epoch `i` is in the borrows set, 
+  then `i` is less than or equal to the high water mark
+*)
+val perm (#v:Type)
+         (#c:Type)
+         (#vp:M.epoch_id -> v -> c -> vprop)
+         (t:tbl vp)
+         (default_value: c)
+         ([@@@smt_fallback] m:repr c)
+         ([@@@smt_fallback] b:borrows v)
+  : vprop
+
+[@@__steel_reduce__; __reduce__]
+let full_perm (#v:Type)
+              (#c:Type)
+              (#vp:M.epoch_id -> v -> c -> vprop)
+              (t:tbl vp)
+              (default_value: c)              
+              ([@@@smt_fallback] m:repr c)
+  = perm t default_value m empty_borrows
+
+(* initializes the EHT and sets high-water-mark to 0 *)
+val create (#v:Type)
+           (#c:Type)
+           (#vp:M.epoch_id -> v -> c -> vprop)
+           (n:U32.t{U32.v n > 0})
+           (init:G.erased c)
+  : STT (tbl #v #c vp)
+        emp
+        (fun a -> perm a init (Map.const #M.epoch_id #c init) empty_borrows)
+
+(* Call the finalizer on the array only.
+   Freeing every element of the array is up to the client *)
+val free (#v:Type)
+         (#c:Type)
+         (#vp:M.epoch_id -> v -> c -> vprop)
+         (#init:G.erased c)
+         (#m:G.erased (repr c))
+         (#b:G.erased (borrows v))
+         (t:tbl vp)
+  : STT unit
+        (perm t init m b)
+        (fun _ -> emp)
+
+noeq
+type get_result (v:Type) =
+  | Found    : v -> get_result v
+  | Fresh    : get_result v
+  | NotFound : get_result v
+
+let get_post
+         (#v:Type) 
+         (#c:Type)
+         (#vp:M.epoch_id -> v -> c -> vprop)
+         (init:G.erased c)
+         (m:G.erased (repr c))
+         (b:G.erased (borrows v))
+         (a:tbl vp)
+         (i:M.epoch_id)
+  : get_result v -> vprop
+  = fun o ->
+    match o with
+    | Found x ->
+      perm a init m (PartialMap.upd i x b)  //when `get` succeeds, the key is added to `borrows`
+        `star`
+      vp i x (Map.sel m i)      //in addition, we return the vp permission for the key
+
+    | _ ->
+      perm a init m b
+
+(*
+   tests if i > high-water-mark; if so it immediately returns Fresh.
+   Otherwise, it looks for epoch i in the EHT
+     - if EHT returns Missing or Absent, return NotFound
+     - Otherwise return Found
+*)     
+val get (#v:Type) 
+        (#c:Type)
+        (#vp:M.epoch_id -> v -> c -> vprop)
+        (#init:G.erased c)
+        (#m:G.erased (repr c))
+        (#b:G.erased (borrows v))
+        (a:tbl vp)
+        (i:M.epoch_id)
+  : ST (get_result v)
+       (perm a init m b)
+       (get_post init m b a i)
+       (requires ~ (PartialMap.contains i b))
+       (ensures fun res -> Fresh? res ==> Map.sel m i == G.reveal init) //<-- This is the main new property
+
+(* Calls EHT.put and moves the high-water-mark to i *)
+val put (#v:Type) 
+        (#c:Type)
+        (#vp:M.epoch_id -> v -> c -> vprop)
+        (#init:G.erased c)
+        (#m:G.erased (repr c))
+        (#b:G.erased (borrows v))
+        (a:tbl vp)
+        (i:M.epoch_id)
+        (x:v)
+        (content:Ghost.erased c)
+  : STT unit
+      (perm a init m b `star` vp i x content)
+      (fun _ -> perm a init (Map.upd m i content) (PartialMap.remove i b))
+
+(* Calls EHT.ghost_put
+   High water mark does not need to be updated, since `i` is in the borrows map *)
+val ghost_put (#o:_)
+              (#v:Type) 
+              (#c:Type)
+              (#vp:M.epoch_id -> v -> c -> vprop)
+              (#init:G.erased c)
+              (#m:G.erased (repr c))
+              (#b:G.erased (borrows v))
+              (a:tbl vp)
+              (i:M.epoch_id)
+              (x:v)
+              (content:Ghost.erased c)
+  : STGhost unit o
+      (perm a init m b `star` vp i x content)
+      (fun _ -> perm a init (Map.upd m i content) (PartialMap.remove i b))
+      (requires
+        PartialMap.sel i b == Some x)
+      (ensures fun _ ->
+        True)
+
+(* This marks a slot in the underlying EHT as being free to reuse, 
+   indicating that the value (if borrowed) will never be returned *)
+val reclaim (#v:Type) 
+            (#c:Type)
+            (#vp:M.epoch_id -> v -> c -> vprop)
+            (#init:G.erased c)
+            (#m:G.erased (repr c))
+            (#b:G.erased (borrows v))
+            (a:tbl vp)
+            (i:M.epoch_id)
+  : STT unit
+      (perm a init m b)
+      (fun _ -> perm a init m (PartialMap.remove i b))
