steel/Zeta.Steel.ThreadStateModel.fst
@@ -55,7 +55,7 @@ let init_epoch_hash =  {
   hadd = HA.initial_hash;
   hevict = HA.initial_hash;
 }
-let epoch_hashes = Zeta.Steel.IArray.repr epoch_id epoch_hash
+let epoch_hashes = m:Map.t epoch_id epoch_hash{ Map.domain m `Set.equal` Set.complement Set.empty }
 let initial_epoch_hashes : epoch_hashes = Map.const init_epoch_hash
 let app_results =
   Seq.seq (fid:A.appfn_id aprm &
